ulib/FStar.Reflection.Arith.fst
@@ -101,7 +101,7 @@ let liftM3 f x y z =
     return (f xx yy zz)
 
 
-private let rec find_idx (f : 'a -> bool) (l : list 'a) : option ((n:nat{n < List.Tot.Base.length l}) * 'a) =
+private let rec find_idx (f : 'a -> Tac bool) (l : list 'a) : Tac (option ((n:nat{n < List.Tot.Base.length l}) * 'a)) =
     match l with
     | [] -> None
     | x::xs ->
@@ -113,7 +113,7 @@ private let rec find_idx (f : 'a -> bool) (l : list 'a) : option ((n:nat{n < Lis
              end
 
 private let atom (t:term) : tm expr = fun (n, atoms) ->
-    match find_idx (term_eq t) atoms with
+    match find_idx (term_eq' t) atoms with
     | None -> Inr (Atom n t, (n + 1, t::atoms))
     | Some (i, t) -> Inr (Atom (n - 1 - i) t, (n, atoms))
 
